@prefix rdf: <http://www.w3.org/1999/02/22-rdf-syntax-ns#> .
@prefix rdfs: <http://www.w3.org/2000/01/rdf-schema#> .
@prefix foaf: <http://xmlns.com/foaf/0.1/> .

# CONCEPTS (CLASSES)
# They are abstractions of the domain.

<#Greenhouse>
    a rdfs:Class ;
    rdfs:label "Greenhouse (Brittany)", "Serra (Brittany)"@it ;
    rdfs:comment "A greenhouse in which the \"Brittany\" software is used.", "Una serra in cui viene utilizzato il software \"Brittany\"."@it ;
    rdfs:seeAlso "https://github.com/Tale152/brittany" .

<#Monitorable>
    a rdfs:Class ;
    rdfs:label "Monitorable (Brittany)", "Monitorabile (Brittany)"@it ;
    rdfs:comment "A space or area that can be monitored by an Edge device.", "Uno spazio o un'area che può essere monitorata da un dispositivo Edge"@it .

<#Environment>
    rdfs:subClassOf <#Monitorable> ;
    rdfs:label "Environment (Brittany)", "Ambiente (Brittany)"@it ;
    rdfs:comment "Section of a Greenhouse in which the \"Brittany\" software is used. An Environment contains Plants. A greenhouse is composed of at least one Environment.", "Sezione di una Serra in cui viene utilizzato il software \"Brittany\". Un ambiente contiene delle piante. Una serra è composta da almeno un Ambiente."@it .

<#Plant>
    rdfs:subClassOf <#Monitorable> ;
    rdfs:label "Plant (Brittany)", "Pianta (Brittany)"@it ;
    rdfs:comment "Vegetal unit contained in an Environment in the Greenhouse", "Unità vegetale contenuta all’interno di un Ambiente della Serra."@it .

<#Edge>
    a rdfs:Class ;
    rdfs:label "Edge (Brittany)", "Edge (Brittany)"@it ;
    rdfs:comment "A digital electronic machine that collect data from Sensor and can manipulate Actuators. An Edge in composed by Modules. An Edge can be placed in an Ambient or on a Plant.", "Una macchina elettronica che colleziona dati dai Sensori e che può manipolare degli Attuatori. Un Edge è composto da Moduli. Un Edge può essere posizionato in un Ambiente o su una Pianta."@it .

<#Module>
    a rdfs:Class ;
    rdfs:label "Module (Brittany)", "Modulo (Brittany)"@it ;
    rdfs:comment "A logical component that can be added to an Edge and is made of OperationHandlers.", "Un componente logico che può essere aggiunto ad un Edge ed è composto da OperationHandlers."@it .

<#OperationHandler>
    a rdfs:Class ;
    rdfs:label "Operation Handler (Brittany)", "Operation Handler (Brittany)"@it ;
    rdfs:comment "An operation that uses some arguments for a computation and returns an result.", "Un'operazione che utilizza degli argomenti per della computazione e ritorna un risultato."@it .

<#ActionOperationHandler>
    rdfs:subClassOf <#OperationHandler> ;
    rdfs:label "Action Operation Handler (Brittany)", "Action Operation Handler (Brittany)"@it ;
    rdfs:comment "An Operation Handler specifically used to execute an Action.", "Un Operation Handler specificatamente utilizzato per eseguire un Azione."@it .

<#PropertyOperationHandler>
    rdfs:subClassOf <#OperationHandler> ;
    rdfs:label "Property Operation Handler (Brittany)", "Property Operation Handler (Brittany)"@it ;
    rdfs:comment "An Operation Handler specifically used to retrieve a Property.", "Un Operation Handler specificatamente utilizzato per recuperare una Properietà."@it .

# RELATIONSHIPS (PROPERTIES)
# They define the existence of relationship between Concepts of the domain.

# TODO Add constraint:
# - only <#Environment> instances are allowed in rdf:range.
# - at least one environment is needed.
<#environments>
    a rdf:Property ;
    rdf:domain <#Greenhouse> ;
    rdf:range rdf:Alt ;
    rdfs:label "Greenhouse contains Environments (Brittany)", "Serra contiene Ambienti (Brittany)"@it ;
    rdfs:comment "Composition property used to indicate that a Greenhouse is composed by one or more Environment.", "Proprietà di composizione utilizzata per indicare che una Serra è composta da uno o più Ambienti."@it .

# TODO Add constraint:
# - only <#BrittanyPlant> instances are allowed in rdf:range.
<#plants>
    a rdf:Property ;
    rdf:domain <#Environment> ;
    rdf:range rdf:Alt ;
    rdfs:label "Environment contains Plants (Brittany)", "Ambiente contiene Piante (Brittany)"@it ;
    rdfs:comment "Composition property used to indicate that a Environments may contains Plants.", "Proprietà di composizione utilizzata per indicare che un Ambiente può contenere Piante."@it .

<#monitor>
    a rdf:Property ;
    rdf:domain <#Edge> ;
    rdf:range <#Monitorable> ;
    rdfs:label "Monitor (Brittany)", "Monitor (Brittany)"@it ;
    rdfs:comment "Property that indicates that an Edge device is placed in a Monitorable area.", "Proprietà che indica che un Edge è posizionato in un area Monitorabile."@it .

<#monitorPlant>
    rdfs:subPropertyOf <#monitor> ;
    rdf:range <#Plant> ;
    rdfs:label "Monitor Plant (Brittany)", "Monitor Pianta (Brittany)"@it ;
    rdfs:comment "Property that indicates that an Edge device is placed on a Plant.", "Proprietà che indica che un Edge è posizionato su una Pianta."@it .

<#monitorEnvironment>
    rdfs:subPropertyOf <#monitor> ;
    rdf:range <#Environment> ;
    rdfs:label "Monitor Environment (Brittany)", "Monitor Ambiente (Brittany)"@it ;
    rdfs:comment "Property that indicates that an Edge device is placed in an Environment.", "Proprietà che indica che un Edge è posizionato in un Ambiente."@it .

# TODO Add constraint:
# - only <#Module> instances are allowed in rdf:range.
# - at least one module is needed.
<#modules>
    a rdf:Property ;
    rdf:domain <#Edge> ;
    rdf:range rdf:Alt ;
    rdfs:label "Module in Edge (Brittany)", "Moduli in Edge (Brittany)"@it ;
    rdfs:comment "Composition property used to indicate that an Edge is composed by one or more Modules.", "Proprietà di composizione utilizzata per indicare che un Edge è composto da uno o più Moduli."@it .

# TODO Add constraint:
# - only <#OperationHandler> instances are allowed in rdf:range.
# - at least one operation handler is needed.
<#handlers>
    a rdf:Property ;
    rdf:domain <#Module> ;
    rdf:range rdf:Alt ;
    rdfs:label "Operation Handlers in Module (Brittany)", "Operation Handlers in Modulo (Brittany)"@it ;
    rdfs:comment "Composition property used to indicate that a Module is composed by one or more Operation Handlers.", "Proprietà di composizione utilizzata per indicare che un Modulo è composto da uno o più Operation Handler."@it .

# INDIVIDUALS
# Elements of the set defined by Concepts.

<#angelo-greenhouse>
    a <#Greenhouse> ;
    foaf:name "Angelo's Greenhouse", "La serra di Angelo"@it ;
    <#environments> [
        a rdf:Alt ;
        rdf:_1 <#angelo-environment>
    ].

<#angelo-environment>
    a <#Environment> ;
    foaf:name "Angelo's Environment #1", "Ambiente di Angelo #1"@it ;
    <#plants> [
        a rdf:Alt ;
        rdf:_1 <#angelo-basil>
    ].

<#angelo-basil>
    a <#Plant> ;
    foaf:name "Angelo's Basil", "Basilico di Angelo"@it .

<angelo-edge>
    a <#Edge> ;
    foaf:name "Angelo's ESP8266", "ESP8266 di Angelo"@it .

# FACTS
# Two Individuals linked by a Relationship.
